project/relational_graph.v
@@ -1,82 +1,52 @@
 Require Import Coq.Relations.Relation_Definitions.
 Require Import Coq.Sets.Ensembles.
+
 (* Defining a Relational Graph *)
 
-Print relation.
-
-(* Definition Powerset : Type -> Type :=
-    fun X => X -> Prop. *)
-
-Definition my_Finite_Type : (Ensemble nat) := 
-    fun X => (X = 0) \/ (X = 1) \/ (X = 2) .
 
     
 Definition valid_cond {t : Type} (nodes : Ensemble t) (rel : relation t) : Type :=
     forall (x y : t), rel x y -> nodes x /\ nodes y.
 
 Record RG (t : Type) := {
-    gr_nodes : Ensemble t;
-    gr_edges : relation t;
-    gr_valid : valid_cond gr_nodes gr_edges
+    RG_nodes : Ensemble t;
+    RG_edges : relation t;
+    RG_valid : valid_cond RG_nodes RG_edges
 }.
 
-Arguments gr_nodes {t}.
-Arguments gr_edges {t}.
-Arguments gr_valid {t}.
-
-
-Definition my_Basic_Graph : RG nat.
-Proof.
-  refine ({|
-    gr_nodes := my_Finite_Type;
-    gr_edges := (fun (A B : nat) => ((A = 0) /\ (B = 1)) \/ 
-                                    ((A = 1) /\ (B = 2)));
-    gr_valid := _
-  |}).
-  unfold valid_cond. intros. split; unfold my_Finite_Type.
-  - destruct H.
-    + left. apply H.
-    + right. left. apply H. 
-  - destruct H.
-    + right. left. apply H.
-    + right. right. apply H.
-Defined.
-
-
-Print my_Basic_Graph.
-
-Compute my_Basic_Graph.(gr_nodes).
-Compute my_Basic_Graph.(gr_edges).
+Arguments RG_nodes {t}.
+Arguments RG_edges {t}.
+Arguments RG_valid {t}.
 
 
 (* Two record graphs are "the same", when their Ensemble and relation are the same *)
-Definition equiv_G {X : Type} (rg1 rg2 : RG X) : Prop :=
+Definition RG_equiv {X : Type} (rg1 rg2 : RG X) : Prop :=
 (* The first condition is definitely needed, as we can have "singleton" graphs *)
-(forall (x : X), rg1.(gr_nodes) x <-> rg2.(gr_nodes) x)
-/\ (forall (x y : X), rg1.(gr_edges) x y <-> rg2.(gr_edges) x y)
+(forall (x : X), rg1.(RG_nodes) x <-> rg2.(RG_nodes) x)
+/\ (forall (x y : X), rg1.(RG_edges) x y <-> rg2.(RG_edges) x y)
 .
-Notation "g1 === g2" := (equiv_G g1 g2) (at level 100, right associativity).
+Notation "g1 === g2" := (RG_equiv g1 g2) (at level 100, right associativity).
 
 
 
-(* "equiv_G" is an equivalence relation: *)
+(* "RG_equiv" is an equivalence relation: *)
 (* Reflexive *)
-Theorem RG_equiv_G_Reflexive {X : Type}: forall (x : RG X), equiv_G x x .
+Theorem RG_RG_equiv_Reflexive {X : Type}: forall (x : RG X), RG_equiv x x .
 Proof.
-    unfold equiv_G. intros. split; split; auto.
+    unfold RG_equiv. intros. split; split; auto.
 Qed.
     
 
 (* Symmetric *)
-Theorem RG_equiv_G_Symmetric {X : Type}: forall (x y : RG X), equiv_G x y <-> equiv_G y x.
+Theorem RG_RG_equiv_Symmetric {X : Type}: forall (x y : RG X), RG_equiv x y <-> RG_equiv y x.
 Proof.
-    split; split; split; unfold equiv_G in H; apply H.
+    split; split; split; unfold RG_equiv in H; apply H.
 Qed. 
 
 (* Transitive *)
-Theorem RG_equiv_G_Transitive {X : Type}: forall (x y z : RG X), equiv_G x y -> equiv_G y z -> equiv_G x z.
+Theorem RG_RG_equiv_Transitive {X : Type}: forall (x y z : RG X), RG_equiv x y -> RG_equiv y z -> RG_equiv x z.
 Proof.
-    split; split; intros; unfold equiv_G in H; unfold equiv_G in H0.
+    split; split; intros; unfold RG_equiv in H; unfold RG_equiv in H0.
     - apply H0. apply H. apply H1.
     - apply H. apply H0. apply H1.
     - apply H0. apply H. apply H1.
@@ -87,12 +57,12 @@ Qed.
 
 (* Source for rewrite: https://stackoverflow.com/questions/56099646/use-rewrite-tactic-with-my-own-operator-in-coq *)
 Require Import Setoid Morphisms.
-Instance RG_Equivalence_eq {X : Type} : Equivalence (@equiv_G X).
+Instance RG_Equivalence_eq {X : Type} : Equivalence (@RG_equiv X).
 Proof.
-    unfold equiv_G. split.
-    - unfold Reflexive. intros. pose proof (@RG_equiv_G_Reflexive X). apply H.
-    - unfold Symmetric. intros. pose proof (@RG_equiv_G_Symmetric X). apply H0. apply H.
-    - unfold Transitive. intros. pose proof (@RG_equiv_G_Transitive X). apply (H1 x y).
+    unfold RG_equiv. split.
+    - unfold Reflexive. intros. pose proof (@RG_RG_equiv_Reflexive X). apply H.
+    - unfold Symmetric. intros. pose proof (@RG_RG_equiv_Symmetric X). apply H0. apply H.
+    - unfold Transitive. intros. pose proof (@RG_RG_equiv_Transitive X). apply (H1 x y).
         + apply H.
         + apply H0.
 Qed.
@@ -102,60 +72,60 @@ Qed.
 Definition RG_empty {A : Type} : RG A.
 Proof.
     refine {|
-        gr_nodes := fun A => False;
-        gr_edges := fun A B => False;
-        gr_valid := _
+        RG_nodes := fun A => False;
+        RG_edges := fun A B => False;
+        RG_valid := _
     |}.
     unfold valid_cond. intros. destruct H.
 Defined.
 
 Definition RG_isEmpty {A : Type} (rg : RG A) : Prop :=
-    forall (a : A), rg.(gr_nodes) a = False
+    forall (a : A), rg.(RG_nodes) a = False
 .
 
 Definition RG_addNode {A : Type} (node : A) (rg : RG A) : RG A.
 Proof.
     refine {|
-        gr_nodes := fun a => node = a \/ rg.(gr_nodes) a;
-        gr_edges := rg.(gr_edges);
-        gr_valid := _
+        RG_nodes := fun a => node = a \/ rg.(RG_nodes) a;
+        RG_edges := rg.(RG_edges);
+        RG_valid := _
     |}.    
     unfold valid_cond. intros. split.
-    - pose proof rg.(gr_valid). unfold valid_cond in X. apply X in H. right. apply H.
-    - pose proof rg.(gr_valid). unfold valid_cond in X. apply X in H. right. apply H.
+    - pose proof rg.(RG_valid). unfold valid_cond in X. apply X in H. right. apply H.
+    - pose proof rg.(RG_valid). unfold valid_cond in X. apply X in H. right. apply H.
 Defined.
 
 Definition RG_addEdge {A : Type} (from to : A) (rg : RG A) : RG A.
 Proof.
     refine {|
-        gr_nodes := fun a => (RG_addNode to (RG_addNode from rg)).(gr_nodes) a;
-        gr_edges := fun a1 a2 => (a1 = from /\ a2 = to) \/ rg.(gr_edges) a1 a2;
-        gr_valid := _
+        RG_nodes := fun a => (RG_addNode to (RG_addNode from rg)).(RG_nodes) a;
+        RG_edges := fun a1 a2 => (a1 = from /\ a2 = to) \/ rg.(RG_edges) a1 a2;
+        RG_valid := _
     |}.    
     unfold valid_cond. simpl. intros. split.
     - destruct H.
         + right. left. destruct H. auto.
-        + right. right. pose proof rg.(gr_valid). unfold valid_cond in X. apply X in H. apply H.
+        + right. right. pose proof rg.(RG_valid). unfold valid_cond in X. apply X in H. apply H.
     - destruct H.
         + left. destruct H. auto.
-        + right. right. pose proof rg.(gr_valid). unfold valid_cond in X. apply X in H. apply H.
+        + right. right. pose proof rg.(RG_valid). unfold valid_cond in X. apply X in H. apply H.
 Qed.
 
 (* Also removes all associated edges *)
 Definition RG_removeNode {A : Type} (node : A) (rg : RG A) : RG A.
 Proof.
     refine {|
-        gr_nodes := fun a => node <> a /\ rg.(gr_nodes) a;
-        gr_edges := fun a1 a2 => node <> a1 /\ node <> a2 /\ rg.(gr_edges) a1 a2;
-        gr_valid := _
+        RG_nodes := fun a => node <> a /\ rg.(RG_nodes) a;
+        RG_edges := fun a1 a2 => node <> a1 /\ node <> a2 /\ rg.(RG_edges) a1 a2;
+        RG_valid := _
     |}.    
     unfold valid_cond. intros. split.
     - split.
         + apply H.
-        + destruct H as [? [? ?]]. pose proof rg.(gr_valid). unfold valid_cond in X. apply X in H1. apply H1.
+        + destruct H as [? [? ?]]. pose proof rg.(RG_valid). unfold valid_cond in X. apply X in H1. apply H1.
     - split.
         + apply H.
-        + destruct H as [? [? ?]]. pose proof rg.(gr_valid). unfold valid_cond in X. apply X in H1. apply H1.
+        + destruct H as [? [? ?]]. pose proof rg.(RG_valid). unfold valid_cond in X. apply X in H1. apply H1.
 Qed.
 
 
@@ -163,22 +133,22 @@ Qed.
 Definition RG_removeEdge {A : Type} (from to : A) (rg : RG A) : RG A.
 Proof.
     refine {|
-        gr_nodes := rg.(gr_nodes);
-        gr_edges := fun a1 a2 => from <> a1 /\ to <> a2 /\ rg.(gr_edges) a1 a2;
-        gr_valid := _
+        RG_nodes := rg.(RG_nodes);
+        RG_edges := fun a1 a2 => from <> a1 /\ to <> a2 /\ rg.(RG_edges) a1 a2;
+        RG_valid := _
     |}.    
     unfold valid_cond. intros. destruct H as [? [? ?]]. split.
-    - pose proof rg.(gr_valid). unfold valid_cond in X. apply X in H1. apply H1.
-    - pose proof rg.(gr_valid). unfold valid_cond in X. apply X in H1. apply H1.
+    - pose proof rg.(RG_valid). unfold valid_cond in X. apply X in H1. apply H1.
+    - pose proof rg.(RG_valid). unfold valid_cond in X. apply X in H1. apply H1.
 Qed.
 
 
 
 Definition RG_getOutgoingEdges {A : Type} (node : A) (rg : RG A) : relation A :=
-    fun (a1 a2 : A) => rg.(gr_edges) a1 a2 /\ a1 = node.
+    fun (a1 a2 : A) => rg.(RG_edges) a1 a2 /\ a1 = node.
 
 Definition RG_getIncomingEdges {A : Type} (node : A) (rg : RG A) : relation A :=
-    fun (a1 a2 : A) => rg.(gr_edges) a1 a2 /\ a2 = node.
+    fun (a1 a2 : A) => rg.(RG_edges) a1 a2 /\ a2 = node.
 
 Definition RG_getIncidentEdges {A : Type} (node : A) (rg : RG A) : relation A :=
     fun (a1 a2 : A) => (RG_getOutgoingEdges node rg) a1 a2 \/ (RG_getIncomingEdges node rg) a1 a2.
@@ -187,22 +157,8 @@ Definition RG_getIncidentEdges {A : Type} (node : A) (rg : RG A) : relation A :=
 
 Require Import Coq.Relations.Relation_Operators.
 Definition RG_existsPath {A : Type} (node1 node2 : A) (rg : RG A) : Prop :=
-    clos_trans A rg.(gr_edges) node1 node2.
+    clos_trans A rg.(RG_edges) node1 node2.
 
-(* 0 -> 1 -> 2 *)
-
-Example RG_existsPath_example : RG_existsPath 0 1 my_Basic_Graph.
-Proof.
-    compute. apply t_step. auto.
-Qed.
-
-(* 0 -> 1 -> 2 *)
-Example RG_existsPath_example' : RG_existsPath 0 2 my_Basic_Graph.
-Proof.
-    compute. apply (t_trans _ _ _ 1).
-    - apply t_step. auto.
-    - apply t_step. auto.
-Qed.
 
 (* Start implementing search *)
 
