project/scrapped_examples/examples.v
@@ -1,0 +1,50 @@
+Require Import Coq.Sets.Ensembles.
+
+Require Import MyProject.project.relational_graph.
+
+(* Mini examples, I had in other files but I moved here for cleanness *)
+
+(* Definition Powerset : Type -> Type :=
+    fun X => X -> Prop. *)
+
+Definition my_Finite_Type : (Ensemble nat) := 
+    fun X => (X = 0) \/ (X = 1) \/ (X = 2) .
+
+
+Definition my_Basic_Graph : RG nat.
+Proof.
+  refine ({|
+    RG_nodes := my_Finite_Type;
+    RG_edges := (fun (A B : nat) => ((A = 0) /\ (B = 1)) \/ 
+                                    ((A = 1) /\ (B = 2)));
+    RG_valid := _
+  |}).
+  unfold valid_cond. intros. split; unfold my_Finite_Type.
+  - destruct H.
+    + left. apply H.
+    + right. left. apply H. 
+  - destruct H.
+    + right. left. apply H.
+    + right. right. apply H.
+Defined.
+
+
+Print my_Basic_Graph.
+
+Compute my_Basic_Graph.(RG_nodes).
+Compute my_Basic_Graph.(RG_edges).
+
+(* 0 -> 1 -> 2 *)
+
+Example RG_existsPath_example : RG_existsPath 0 1 my_Basic_Graph.
+Proof.
+    compute. apply t_step. auto.
+Qed.
+
+(* 0 -> 1 -> 2 *)
+Example RG_existsPath_example' : RG_existsPath 0 2 my_Basic_Graph.
+Proof.
+    compute. apply (t_trans _ _ _ 1).
+    - apply t_step. auto.
+    - apply t_step. auto.
+Qed.
